Splinter/Journal/LinkedJournalRefinement.i.dfy
@@ -33,11 +33,12 @@ module LinkedJournalRefinement
     requires dv2.WF() && dv2.Acyclic() && dv2.PointersRespectRank(r2)
     requires dv1.IsNondanglingPointer(ptr)
     requires dv1.IsSubDisk(dv2)
+    requires dv1.boundaryLSN == dv2.boundaryLSN
     ensures dv1.RankedIPtr(ptr, r1) == dv2.RankedIPtr(ptr, r2)
     decreases if ptr.Some? then r1[ptr.value] else -1
   {
-    if ptr != None {
-      RankedIPtrFraming(dv1, dv2, r1, r2, dv1.CroppedPointer(dv1.entries[ptr.value].priorRec));
+    if ptr.Some? {
+      RankedIPtrFraming(dv1, dv2, r1, r2, dv1.entries[ptr.value].CroppedPrior(dv1.boundaryLSN));
     }
   }
 
@@ -46,6 +47,7 @@ module LinkedJournalRefinement
     requires dv2.WF() && dv2.Acyclic()
     requires dv1.IsNondanglingPointer(ptr)
     requires dv1.IsSubDisk(dv2)
+    requires dv1.boundaryLSN == dv2.boundaryLSN
     ensures dv1.IPtr(ptr) == dv2.IPtr(ptr)
   {
     RankedIPtrFraming(dv1, dv2, dv1.TheRanking(), dv2.TheRanking(), ptr);
@@ -70,18 +72,6 @@ module LinkedJournalRefinement
   {
   }
 
-  lemma DiscardOldPreservesAcyclic(big: DiskView, cropped: DiskView)
-    requires big.WF()
-    requires big.boundaryLSN <= cropped.boundaryLSN
-    requires big.Acyclic()
-    requires cropped == big.DiscardOld(cropped.boundaryLSN)
-    ensures cropped.WF()
-    ensures cropped.Acyclic()
-  {
-    var ranking :| big.PointersRespectRank(ranking);
-    assert cropped.PointersRespectRank(ranking);
-  }
-
   lemma DiscardInterp(dv: DiskView, lsn: LSN, discarded: DiskView, ptr: Pointer)
     requires dv.WF()
     requires dv.Acyclic()
@@ -92,27 +82,30 @@ module LinkedJournalRefinement
     ensures discarded.RankedIPtr(ptr, discarded.TheRanking()) == PagedJournal.DiscardOldJournalRec(dv.IPtr(ptr), lsn)
     decreases if ptr.Some? then dv.TheRanking()[ptr.value] else -1
   {
-    DiscardOldPreservesAcyclic(dv, discarded);
-    if !ptr.None? {
-      if dv.entries[ptr.value].messageSeq.seqEnd <= lsn {
-        assert discarded.RankedIPtr(ptr, discarded.TheRanking()).None?;
-        assert PagedJournal.DiscardOldJournalRec(dv.IPtr(ptr), lsn).None?;
-        assert discarded.RankedIPtr(ptr, discarded.TheRanking()) == PagedJournal.DiscardOldJournalRec(dv.IPtr(ptr), lsn);
-      } else {
-        DiscardInterp(dv, lsn, discarded, dv.CroppedPointer(dv.entries[ptr.value].priorRec));
-        if dv.entries[ptr.value].messageSeq.seqStart <= lsn {
-          assert discarded.RankedIPtr(ptr, discarded.TheRanking()).value.priorRec.None?;
-          assert PagedJournal.DiscardOldJournalRec(dv.IPtr(ptr), lsn).value.priorRec.None?;
-          assert discarded.RankedIPtr(ptr, discarded.TheRanking()) == PagedJournal.DiscardOldJournalRec(dv.IPtr(ptr), lsn);
-        } else {
-          assert discarded.RankedIPtr(ptr, discarded.TheRanking()) == PagedJournal.DiscardOldJournalRec(dv.IPtr(ptr), lsn);
-        }
-      }
+    assert discarded.PointersRespectRank(dv.TheRanking());
+    if ptr.Some? && !(dv.entries[ptr.value].messageSeq.seqStart <= lsn) {
+      DiscardInterp(dv, lsn, discarded, discarded.entries[ptr.value].CroppedPrior(discarded.boundaryLSN));
     }
   }
     
-//    ensures 
-
+  lemma SubDiskInterp(small: DiskView, big: DiskView, ptr: Pointer)
+    requires big.WF()
+    requires big.Acyclic()
+    requires small.WF()
+    requires small.IsSubDisk(big)
+    requires small.boundaryLSN == big.boundaryLSN
+    requires small.IsNondanglingPointer(ptr)
+    ensures small.Acyclic()
+    ensures small.RankedIPtr(ptr, small.TheRanking()) == big.RankedIPtr(ptr, big.TheRanking())
+    decreases if ptr.Some? then big.TheRanking()[ptr.value] else -1
+  {
+    assert small.PointersRespectRank(big.TheRanking());
+    if ptr.Some? {
+      var jr := big.entries[ptr.value];
+      SubDiskInterp(small, big, jr.CroppedPrior(big.boundaryLSN));
+    }
+  }
+    
   lemma InvNext(v: Variables, v': Variables, lbl: TransitionLabel)
     requires Inv(v)
     requires Next(v, v', lbl)
@@ -128,46 +121,17 @@ module LinkedJournalRefinement
     } else if step.PutStep? {
       assert Inv(v');
     } else if step.DiscardOldStep? {
-      assert DiskView(v.truncatedJournal.diskView.boundaryLSN, map[]).PointersRespectRank(map[]);  // need ranking for case where we make a fresh empty diskview
-
       var lsn := lbl.startLsn;
       var croppedTJ := v.truncatedJournal.DiscardOld(lbl.startLsn);
-      if v.unmarshalledTail.seqStart <= lsn {
-        // TODO(jonh): turn on tight before eliminating this proof
-        assert croppedTJ.freshestRec == None;
-        assert croppedTJ.diskView == v.truncatedJournal.diskView.DiscardOld(lbl.startLsn);
-        DiscardOldPreservesAcyclic(v.truncatedJournal.diskView, croppedTJ.diskView);
-        assert croppedTJ.diskView.Acyclic();
-        assert croppedTJ.I() == PagedJournal.TruncatedJournal(lsn, None);
-      } else {
-        DiscardOldPreservesAcyclic(v.truncatedJournal.diskView, croppedTJ.diskView);
-        assert v.SeqStart() == v.truncatedJournal.I().I().seqStart
-          by { v.truncatedJournal.I().BuildReceipt().TJFacts(); }
-        if !(v.truncatedJournal.freshestRec.None? 
-          || v.truncatedJournal.diskView.entries[v.truncatedJournal.freshestRec.value].messageSeq.seqEnd <= lsn) {
-          var diskView := v.truncatedJournal.diskView;
-          var discardedDV := diskView.DiscardOld(lsn);
-          calc {
-            TruncatedJournal(v.truncatedJournal.freshestRec, diskView.DiscardOld(lsn)).I().freshestRec;
+      var diskView := v.truncatedJournal.diskView;
 
-            diskView.DiscardOld(lsn).IPtr(v.truncatedJournal.freshestRec);
-            discardedDV.RankedIPtr(v.truncatedJournal.freshestRec, discardedDV.TheRanking());
-              { DiscardInterp(v.truncatedJournal.diskView, lsn, discardedDV, v.truncatedJournal.freshestRec); }
-            
-            PagedJournal.DiscardOldJournalRec(v.truncatedJournal.diskView.IPtr(v.truncatedJournal.freshestRec), lsn);
-            PagedJournal.DiscardOldJournalRec(v.truncatedJournal.I().freshestRec, lsn);
-            v.truncatedJournal.I().DiscardOld(lsn).freshestRec;
-          }
-          calc {
-            croppedTJ.I().freshestRec;
-            TruncatedJournal(v.truncatedJournal.freshestRec, v.truncatedJournal.diskView.DiscardOld(lsn)).I().freshestRec;
-            v.truncatedJournal.I().DiscardOld(lsn).freshestRec;
-          }
-        }
-        assert croppedTJ.I() == v.truncatedJournal.I().DiscardOld(lsn);
+      assert v'.truncatedJournal.diskView.PointersRespectRank(diskView.TheRanking());  // ranking witness gets across both DiscardOld and tightening
+      if !(v.unmarshalledTail.seqStart <= lsn) {
+        assert v.SeqStart() == v.truncatedJournal.I().I().seqStart by { v.truncatedJournal.I().BuildReceipt().TJFacts(); }
+        DiscardInterp(diskView, lsn, diskView.DiscardOld(lsn), v.truncatedJournal.freshestRec);
+        SubDiskInterp(v'.truncatedJournal.diskView, croppedTJ.diskView, croppedTJ.freshestRec);
+        assert croppedTJ.I() == v.truncatedJournal.I().DiscardOld(lsn); // Trigger for v'.I().WF()
       }
-
-      assert PagedJournal.DiscardOld(I(v), I(v'), lbl); // trigger
       assert Inv(v');
     } else if step.InternalJournalMarshalStep? {
       // Witness new rank
@@ -209,28 +173,15 @@ module LinkedJournalRefinement
       assert PagedJournal.NextStep(I(v), I(v'), lbl, PagedJournal.PutStep()); // witness step
     } else if step.DiscardOldStep? {
       var lsn := lbl.startLsn;
-      assume false;
-      if v.unmarshalledTail.seqStart <= lsn {
-        assert I(v').truncatedJournal == PagedJournal.TruncatedJournal(lsn, None);
-      } else {
-        var tj := v.truncatedJournal;
-        var tj' := v'.truncatedJournal;
-        calc {
-          v.SeqStart();
-          v.truncatedJournal.SeqStart();
-          v.truncatedJournal.diskView.boundaryLSN;
-            { assume false; }
-          v.truncatedJournal.I().I().seqStart;  // HERE
-          I(v).truncatedJournal.I().seqStart;
+      if !(v.unmarshalledTail.seqStart <= lsn) {
+        assert v.SeqStart() == I(v).truncatedJournal.I().seqStart by {
+          var tj := v.truncatedJournal;
+          var dv := v.truncatedJournal.diskView;
+          PagedJournal.TruncatedJournal(dv.boundaryLSN, dv.IPtr(tj.freshestRec)).BuildReceipt().TJFacts();
         }
-        assert v.SeqStart() == I(v).truncatedJournal.I().seqStart;
-        assert I(v).truncatedJournal.I().seqStart <= lsn;
-        assert I(v).truncatedJournal.I().CanDiscardTo(lsn);
-        assert I(v').truncatedJournal.boundaryLSN == I(v).truncatedJournal.DiscardOld(lsn).boundaryLSN;
-        assert tj'.diskView.IPtr(tj'.freshestRec) == tj.I().DiscardOld(lsn).freshestRec;
-        assert v'.truncatedJournal.I().freshestRec == v.truncatedJournal.I().DiscardOld(lsn).freshestRec;
-        assert I(v').truncatedJournal.freshestRec == I(v).truncatedJournal.DiscardOld(lsn).freshestRec;
-        assert I(v').truncatedJournal == I(v).truncatedJournal.DiscardOld(lsn);
+        var croppedTJ := v.truncatedJournal.DiscardOld(lbl.startLsn);
+        DiscardInterp(v.truncatedJournal.diskView, lsn, croppedTJ.diskView, v.truncatedJournal.freshestRec);
+        SubDiskInterp(v'.truncatedJournal.diskView, croppedTJ.diskView, croppedTJ.freshestRec);
       }
       assert PagedJournal.NextStep(I(v), I(v'), lbl, PagedJournal.DiscardOldStep()); // witness step
     } else if step.InternalJournalMarshalStep? {
